Cleanup in quicksort.

HOL/DataStrs/Quicksort.thy
@@ -7,20 +7,18 @@ section {* Outer remains *}
 definition outer_remains :: "'a list \<Rightarrow> 'a list \<Rightarrow> nat \<Rightarrow> nat \<Rightarrow> bool" where [rewrite]:
   "outer_remains xs xs' l r \<longleftrightarrow> (length xs = length xs' \<and> (\<forall>i. i < l \<or> r < i \<longrightarrow> xs ! i = xs' ! i))"
 
-lemma outer_remainsD1: "outer_remains xs xs' l r \<Longrightarrow> i < l \<Longrightarrow> xs ! i = xs' ! i" by auto2
-setup {* add_forward_prfstep_cond @{thm outer_remainsD1} [with_term "?xs' ! ?i"] *}
+lemma outer_remains_length [forward]:
+  "outer_remains xs xs' l r \<Longrightarrow> length xs = length xs'" by auto2
 
-lemma outer_remainsD2: "outer_remains xs xs' l r \<Longrightarrow> r < i \<Longrightarrow> xs ! i = xs' ! i" by auto2
-setup {* add_forward_prfstep_cond @{thm outer_remainsD2} [with_term "?xs' ! ?i"] *}
-  
-lemma outer_remainsD3 [forward]: "outer_remains xs xs' l r \<Longrightarrow> length xs = length xs'" by auto2
+lemma outer_remains_eq [rewrite_back]:
+  "outer_remains xs xs' l r \<Longrightarrow> i < l \<Longrightarrow> xs ! i = xs' ! i"
+  "outer_remains xs xs' l r \<Longrightarrow> r < i \<Longrightarrow> xs ! i = xs' ! i" by auto2+
 
-lemma outer_remainsD_take [rewrite]:
-  "i \<le> length xs \<Longrightarrow> outer_remains xs xs' l r \<Longrightarrow> i < l \<Longrightarrow> take i xs = take i xs'" by auto2
-
-lemma outer_remainsD_drop [rewrite]:
-  "outer_remains xs xs' l r \<Longrightarrow> r < i \<Longrightarrow> drop i xs = drop i xs'" by auto2
-
+lemma outer_remains_sublist [backward2]:
+  "outer_remains xs xs' l r \<Longrightarrow> i < l \<Longrightarrow> take i xs = take i xs'"
+  "outer_remains xs xs' l r \<Longrightarrow> r < i \<Longrightarrow> drop i xs = drop i xs'"
+  "i \<le> j \<Longrightarrow> j \<le> length xs \<Longrightarrow> outer_remains xs xs' l r \<Longrightarrow> j \<le> l \<Longrightarrow> sublist i j xs = sublist i j xs'"
+  "i \<le> j \<Longrightarrow> j \<le> length xs \<Longrightarrow> outer_remains xs xs' l r \<Longrightarrow> i > r \<Longrightarrow> sublist i j xs = sublist i j xs'" by auto2+
 setup {* del_prfstep_thm_eqforward @{thm outer_remains_def} *}
 
 section {* part1 function *}  
@@ -57,7 +55,7 @@ lemma part1_partitions2 [backward]:
 
 section {* Paritition function *}
 
-definition partition :: "('a::linorder list) \<Rightarrow> nat \<Rightarrow> nat \<Rightarrow> (nat \<times> 'a list)" where
+definition partition :: "('a::linorder list) \<Rightarrow> nat \<Rightarrow> nat \<Rightarrow> (nat \<times> 'a list)" where [rewrite]:
   "partition xs l r = (
     let p = xs ! r;
       (m, xs') = part1 xs l (r - 1) p;
@@ -68,76 +66,66 @@ setup {* register_wellform_data ("partition xs l r", ["l < r", "r < length xs"])
 
 lemma partition_basic:
   "l < r \<Longrightarrow> r < length xs \<Longrightarrow> (rs, xs') = partition xs l r \<Longrightarrow>
-   outer_remains xs xs' l r \<and> mset xs' = mset xs \<and> l \<le> rs \<and> rs \<le> r"
-@proof @unfold "partition xs l r" @qed
+   outer_remains xs xs' l r \<and> mset xs' = mset xs \<and> l \<le> rs \<and> rs \<le> r" by auto2
 setup {* add_forward_prfstep_cond @{thm partition_basic} [with_term "partition ?xs ?l ?r"] *}
   
 lemma partition_partitions1 [forward]:
   "l < r \<Longrightarrow> r < length xs \<Longrightarrow> (rs, xs') = partition xs l r \<Longrightarrow>
    x \<in> set (sublist l rs xs') \<Longrightarrow> x \<le> xs' ! rs"
-@proof @unfold "partition xs l r" @obtain i where "i \<ge> l" "i < rs" "x = xs' ! i" @qed
+@proof @obtain i where "i \<ge> l" "i < rs" "x = xs' ! i" @qed
 
 lemma partition_partitions2 [forward]:
   "l < r \<Longrightarrow> r < length xs \<Longrightarrow> (rs, xs'') = partition xs l r \<Longrightarrow>
    x \<in> set (sublist (rs + 1) (r + 1) xs'') \<Longrightarrow> x \<ge> xs'' ! rs"
-@proof @unfold "partition xs l r"
+@proof
   @obtain i where "i \<ge> rs + 1" "i < r + 1" "x = xs'' ! i"
   @let "p = xs ! r"
   @let "m = fst (part1 xs l (r - 1) p)"
   @let "xs' = snd (part1 xs l (r - 1) p)"
   @case "xs' ! m \<le> p"
 @qed
+setup {* del_prfstep_thm @{thm partition_def} *}
 
-lemma quicksort_term1 [resolve]:
+lemma quicksort_term1:
   "l < r \<Longrightarrow> r < length xs \<Longrightarrow> fst (partition xs l r) - (l + 1) < r - l"
 @proof @have "fst (partition xs l r) - l - 1 < r - l" @qed
 
-lemma quicksort_term2 [resolve]:
+lemma quicksort_term2:
   "l < r \<Longrightarrow> r < length xs \<Longrightarrow> r - (fst (partition xs l r) + 1) < r - l"
 @proof @have "r - fst (partition xs l r) - 1 < r - l" @qed
 
 function quicksort :: "('a::linorder) list \<Rightarrow> nat \<Rightarrow> nat \<Rightarrow> 'a list" where
   "quicksort xs l r = (
     if l \<ge> r then xs
-    else if r < length xs then
-      let (p, xs1) = partition xs l r;
-        xs2 = quicksort xs1 l (p - 1)
-      in
-        quicksort xs2 (p + 1) r
-    else xs)"
-  by auto
-  termination apply (relation "measure (\<lambda>(a, l, r). (r - l))")
-  apply auto by auto2+
+    else if r \<ge> length xs then xs
+    else let
+      (p, xs1) = partition xs l r;
+      xs2 = quicksort xs1 l (p - 1)
+    in
+      quicksort xs2 (p + 1) r)"
+  by auto termination apply (relation "measure (\<lambda>(a, l, r). (r - l))") apply auto
+  apply (metis quicksort_term1 Suc_eq_plus1 fst_conv not_le_imp_less)
+  by (metis quicksort_term2 Suc_eq_plus1 fst_conv not_le_imp_less)
 
-lemma quicksort_trivial [rewrite]:
+lemma quicksort_basic [rewrite_arg]:
+  "mset (quicksort xs l r) = mset xs \<and> outer_remains xs (quicksort xs l r) l r"
+@proof @fun_induct "quicksort xs l r" @with
+  @subgoal "(xs = xs, l = l, r = r)"
+    @unfold "quicksort xs l r"
+  @end
+@qed
+
+lemma quicksort_trivial1 [rewrite]:
   "l \<ge> r \<Longrightarrow> quicksort xs l r = xs"
 @proof @unfold "quicksort xs l r" @qed
 
-lemma quicksort_basic:
-  "mset (quicksort xs l r) = mset xs \<and> outer_remains xs (quicksort xs l r) l r"
-@proof
-  @let "d = r - l"
-  @strong_induct d arbitrary l r xs
-  @unfold "quicksort xs l r"
-  @case "l \<ge> r" @case "r \<ge> length xs"
-  @let "p = fst (partition xs l r)"
-  @let "xs1 = snd (partition xs l r)"
-  @let "xs2 = quicksort xs1 l (p - 1)"
-  @let "xs3 = quicksort xs l r"
-  @have "mset xs2 = mset xs1 \<and> outer_remains xs1 xs2 l r" @with
-    @case "p - 1 \<le> l"
-    @apply_induct_hyp "(p-1)-l" l "p-1" xs1
-  @end
-  @have "mset xs3 = mset xs2 \<and> outer_remains xs2 xs3 l r" @with
-    @case "p + 1 \<ge> r"
-    @apply_induct_hyp "r-(p+1)" "p+1" r xs2
-  @end
-@qed
-setup {* add_forward_prfstep_cond @{thm quicksort_basic} [with_term "quicksort ?xs ?l ?r"] *}
+lemma quicksort_trivial2 [rewrite]:
+  "r \<ge> length xs \<Longrightarrow> quicksort xs l r = xs"
+@proof @unfold "quicksort xs l r" @qed
 
-lemma quicksort_permutes [rewrite]:
+lemma quicksort_permutes [resolve]:
   "xs' = quicksort xs l r \<Longrightarrow> set (sublist l (r + 1) xs') = set (sublist l (r + 1) xs)"
-@proof @unfold "quicksort xs l r"
+@proof
   @case "l \<ge> r" @case "r \<ge> length xs"
   @have "xs = take l xs @ sublist l (r + 1) xs @ drop (r + 1) xs"
   @have "xs' = take l xs' @ sublist l (r + 1) xs' @ drop (r + 1) xs'"
@@ -145,42 +133,41 @@ lemma quicksort_permutes [rewrite]:
   @have "drop (r + 1) xs = drop (r + 1) xs'"
 @qed
 
-lemma quicksort_sorts:
-  "r < length xs \<Longrightarrow> sorted (sublist l (r + 1) (quicksort xs l r))"
+lemma sorted_pivoted_list [forward]:
+  "l \<le> p \<Longrightarrow> p + 1 \<le> r \<Longrightarrow> r \<le> length xs \<Longrightarrow>
+   sorted (sublist (p + 1) r xs) \<Longrightarrow> sorted (sublist l p xs) \<Longrightarrow>
+   \<forall>x\<in>set (sublist l p xs). x \<le> xs ! p \<Longrightarrow> \<forall>y\<in>set (sublist (p + 1) r xs). xs ! p \<le> y \<Longrightarrow>
+   sorted (sublist l r xs)"
 @proof
-  @let "d = r - l"
-  @case "l \<ge> r" @case "r \<ge> length xs"
-  @strong_induct d arbitrary l r xs
+  @have "sublist l r xs = sublist l p xs @ (xs ! p) # sublist (p + 1) r xs"
+@qed
+
+lemma quicksort_sorts [forward_arg]:
+  "r < length xs \<Longrightarrow> sorted (sublist l (r + 1) (quicksort xs l r))"
+@proof @fun_induct "quicksort xs l r" @with
+  @subgoal "(xs = xs, l = l, r = r)"
+  @case "l \<ge> r" @with @case "l = r" @end
+  @case "r \<ge> length xs"
   @let "p = fst (partition xs l r)"
   @let "xs1 = snd (partition xs l r)"
   @let "xs2 = quicksort xs1 l (p - 1)"
   @let "xs3 = quicksort xs2 (p + 1) r"
-  @have "xs1 ! p = xs3 ! p"
-  @have "sublist l p xs2 = sublist l p xs3"
-  @have "set (sublist l p xs1) = set (sublist l p xs2)" @with
-    @case "p = 0" @have "p = p - 1 + 1" @end
-  @have "sublist (p + 1) (r + 1) xs1 = sublist (p + 1) (r + 1) xs2"
-  @have "set (sublist (p + 1) (r + 1) xs2) = set (sublist (p + 1) (r + 1) xs3)"
-  @have "\<forall>x\<in>set (sublist l p xs3). x \<le> xs3 ! p"
-  @have "\<forall>x\<in>set (sublist (p + 1) (r + 1) xs1). x \<ge> xs1 ! p"
-  @have "sorted (sublist l p xs3)" @with
-    @case "p = 0"
-    @case "l \<ge> p - 1" @with @have "p = p - 1 + 1" @end
-    @apply_induct_hyp "(p-1)-l" l "p-1" xs1
+  @have "sorted (sublist l (r + 1) xs3)" @with
+    @have "l \<le> p" @have "p + 1 \<le> r + 1" @have "r + 1 \<le> length xs3"
+    @have "sublist l p xs2 = sublist l p xs3"
+    @have "set (sublist l p xs1) = set (sublist l p xs2)"
+    @have "sublist (p + 1) (r + 1) xs1 = sublist (p + 1) (r + 1) xs2"
+    @have "set (sublist (p + 1) (r + 1) xs2) = set (sublist (p + 1) (r + 1) xs3)"
+    @have "\<forall>x\<in>set (sublist l p xs3). x \<le> xs3 ! p"
+    @have "\<forall>x\<in>set (sublist (p + 1) (r + 1) xs3). x \<ge> xs3 ! p"
+    @have "sorted (sublist l p xs3)"
+    @have "sorted (sublist (p + 1) (r + 1) xs3)"
   @end
-  @have "sorted (sublist (p + 1) (r + 1) xs3)" @with
-    @case "r \<le> p + 1"
-    @apply_induct_hyp "r-(p+1)" "p+1" r xs2
-  @end
-  @unfold "quicksort xs l r"
+  @unfold "quicksort xs l r" @end
 @qed
-setup {* add_forward_prfstep_cond @{thm quicksort_sorts} [with_term "quicksort ?xs ?l ?r"] *}
 
 lemma quicksort_sorts_all [rewrite]:
-  "xs \<noteq> [] \<Longrightarrow> quicksort xs 0 (length xs - 1) = sort xs"
-@proof
-  @let "xs' = quicksort xs 0 (length xs - 1)"
-  @have "sublist 0 (length xs) xs' = xs'"
-@qed
+  "xs \<noteq> [] \<Longrightarrow> xs' = quicksort xs 0 (length xs - 1) \<Longrightarrow> xs' = sort xs"
+@proof @have "sublist 0 (length xs - 1 + 1) xs' = xs'" @qed
 
 end
